# descriptions: documents, services
@prefix rdf: <http://www.w3.org/1999/02/22-rdf-syntax-ns#> .
@prefix rdfs: <http://www.w3.org/2000/01/rdf-schema#> .
@prefix owl: <http://www.w3.org/2002/07/owl#> .
@prefix xsd: <http://www.w3.org/2001/XMLSchema#> .
@prefix ptg: <http://protege.stanford.edu/plugins/owl/protege#> .

@prefix prov: <http://www.w3.org/ns/prov#> .
@prefix dc: <http://purl.org/dc/terms/> .
@prefix dctype: <http://purl.org/dc/dcmitype/> .
@prefix skos: <http://www.w3.org/2004/02/skos/core#> .
@prefix foaf: <http://xmlns.com/foaf/0.1/> .
@prefix bibo: <http://purl.org/ontology/bibo/> .

@prefix edtf: <http://id.loc.gov/datatypes/edtf/> .
@prefix bf2: <http://id.loc.gov/ontologies/bibframe/> .
@prefix bflc: <http://id.loc.gov/ontologies/bflc/> .
@prefix sdo: <http://schema.org/> .
@prefix madsrdf: <http://www.loc.gov/mads/rdf/v1#> .

@prefix quid: <https://w3id.org/quid/> .

@prefix : <https://id.kb.se/vocab/> .
@prefix bulk: <https://id.kb.se/ns/bulk/> .

: a owl:Ontology;
    owl:sameAs <https://id.kb.se/vocab> ;
    dc:title "KB Base Vocabulary"@en;
    dc:title "KB:s basvokabulär"@sv;
    rdfs:comment "Detta vokabulär fungerar som en central mappning till publika, välkända egenskaper och klasser."@sv;
    rdfs:comment "This vocabulary serves as a central mapping to public, well-known properties and classes."@en;
    dc:license <http://creativecommons.org/publicdomain/zero/1.0/> ;
    owl:imports dc:, dctype:, skos:, prov:, foaf:, bibo:, sdo:, bf2:, bflc: ;
    skos:hasTopConcept :Instance, :Work, :Item, :Agent, :Concept ;
    :dataDisplay <https://id.kb.se/vocab/display> .


##
# Local Definitions Of Core Vocabulary Components
##
# TODO: just use context aliases, and add these labels in <external-labels.ttl>?

rdf:type a owl:ObjectProperty;
    rdfs:label "type"@en, "typ"@sv .

# TODO: Used for simplified rolification in property chain axioms.
#:selfOfType rdfs:subPropertyOf [ owl:inverseOf owl:onProperty ] ;
#  rdfs:range [ owl:onProperty owl:hasSelf ; owl:hasValue true ] .

:Resource a owl:Class ;
    owl:equivalentClass rdfs:Resource;
    rdfs:label "Resurs"@sv, "Resource"@en;
    skos:altLabel "Entitet"@sv, "Entity"@en .

:Ontology a owl:Class ;
    owl:equivalentClass owl:Ontology ;
    rdfs:subClassOf :Resource;
    rdfs:label "Ontologi"@sv, "Ontology"@en ;
    skos:altLabel "Vokabulär"@sv, "Vocabulary"@en .

:Class a owl:Class;
    owl:equivalentClass owl:Class;
    rdfs:label "Class"@en, "Klass"@sv .

:ObjectProperty a owl:Class;
    owl:equivalentClass owl:ObjectProperty;
    rdfs:label "Object property"@en, "Relation"@sv .

:FunctionalProperty a owl:Class;
    owl:equivalentClass owl:FunctionalProperty;
    rdfs:label "Functional property"@en, "Funktionell egenskap"@sv .

:TransitiveProperty a owl:Class;
    owl:equivalentClass owl:TransitiveProperty;
    rdfs:label "Transitive property"@en, "Transitiv egenskap"@sv .

:SymmetricProperty a owl:Class;
    owl:equivalentClass owl:SymmetricProperty;
    rdfs:subClassOf :ObjectProperty;
    rdfs:label "Symmetric property"@en, "Symmetrisk relation"@sv .

:DatatypeProperty a owl:Class;
    owl:equivalentClass owl:DatatypeProperty;
    rdfs:range :Datatype;
    rdfs:label "Data type property"@en, "Egenskap"@sv .

:Datatype a owl:Class;
    owl:equivalentClass rdfs:Datatype;
    rdfs:label "Data type"@en, "Datatyp"@sv .

##
# Extended Vocabulary Components

:StructuredProperty a owl:Class;
    rdfs:subPropertyOf owl:ObjectProperty;
    rdfs:range :StructuredValue;
    rdfs:label "Structured property"@en,  "Strukturerad egenskap"@sv .

:StructuredValue a owl:Class;
    owl:equivalentClass sdo:StructuredValue;
    rdfs:subClassOf :Resource;
    skos:closeMatch rdfs:Datatype;
    rdfs:label "Structured value"@en, "Strukturerat värde"@sv .


# NOTE: these constructs, used below, will yield inferred statements, which if
# interpreted, will produce direct links using subject of hasStatement,
# predicate(s) from role(s) and object from an object property. Like:
#CONSTRUCT { ?s ?p ?o } WHERE {
#    ?s [rdfs:subPropertyOf? :hasStatement] [
#            [rdfs:subPropertyOf? :predicate] ?p;
#            [rdfs:subPropertyOf? :object] ?o ]
#}

:QualifiedRole a owl:Class;
    rdfs:subClassOf rdf:Statement ;
    ptg:abstract true ;
    owl:equivalentClass sdo:Role;
    rdfs:label "Qualified role"@en, "Kvalificerad roll"@sv .

:hasStatement a owl:ObjectProperty;
    ptg:abstract true;
    rdfs:subPropertyOf [ owl:inverseOf rdf:subject ];
    rdfs:range rdf:Statement .

:predicate a owl:ObjectProperty;
    rdfs:subPropertyOf rdf:predicate; ptg:abstract true .

:object a owl:ObjectProperty;
    rdfs:subPropertyOf rdf:object; ptg:abstract true .


##
# Temporal qualifications (cf. https://en.wikipedia.org/wiki/Perdurantism)
#
# A perdurant entity ("4D worm") has exdurant parts (carrying the properties of
# a "stage"). Temporal entities are somewhere in between ("slices of time").
# Think of them as discrete, statistical things, carrying some properties,
# stable witin that time slice, of something perdurant.
#
# To compare, for *endurant* entities, properties do not change. For instance,
# a newspaper issue had a specific geographical coverage, whereas for the
# newspaper serial, this coverage may change, but probably not for every issue.
# The newspaper issue is, for all practical cataloging purposes, an endurant
# thing, whereas the serial has aspects, such as geographic coverage, which can
# be temporally qualified.

:TemporalEntity a owl:Class ;
    ptg:abstract true ;
    rdfs:label "Temporal entity"@en, "Temporal entitet"@sv;
    rdfs:comment "Something existing over a period of time."@en ;
    rdfs:subClassOf quid:QualifiedIdentity .

:TemporalQualification a owl:Class ;
    ptg:abstract true ;
    rdfs:label "Temporal qualification"@en, "Temporal kvalificering"@sv;
    rdfs:comment "Constitues an aspect of a more distinct entity."@en ;
    rdfs:subClassOf :TemporalEntity, :QualifiedRole .


##
# Categorization (looser typing) of Resources, including Terms

:category a owl:ObjectProperty;
    rdfs:label "category"@en, "kategori"@sv;
    sdo:domainIncludes :ChangeNote, :Work, :Instance ;
    sdo:rangeIncludes :Category, :Genre, :GenreForm, :ContentType ;
    owl:equivalentProperty sdo:category .

:Category a owl:Class ;
    #rdfs:subClassOf :Concept ;
    rdfs:label "Category"@en, "Kategori"@sv .

##
# These terms may also be "bibliographic", but the platform cannot work without
# them. If the "bibliographic" notions are 1:1 with the technical, the term is
# the same, otherwise we need subclasses (which may also derive from other
# subclasses).
# See also: <https://github.com/libris/definitions/pull/413>
:platform a skos:Collection ;
    :code "platform" ;
    rdfs:comment "Terms required by the XL platform."@en .

:shorthand a skos:Collection ;
    rdfs:label "shorthand"@en, "kortform"@sv ;
    rdfs:comment "Anges som kategori på egenskaper som har en mer komplex bakomliggande struktur."@sv ;
    skos:example "Exempelvis isbn, som motsvarar identifiedBy(type=ISBN).value."@sv ;
    skos:scopeNote "Används i Libris katalogiseringsverktyg för att dölja dessa vid listning av egenskaper."@sv ;
    :code "shorthand" .

:compositional a skos:Collection ;
    rdfs:label "compositional"@en, "inneboende del"@sv ;
    rdfs:comment "Anges på egenskaper för att betrakta deras värde som en sammansatt del av entiteten, istället för en länkbar fristående entitet."@sv ;
    skos:example "Exempelvis hasVariant, som anger variantbeskrivingar av en Agent som distinkta Agenter (men enbart i formen, de respresenterar samma ting)."@sv ;
    skos:scopeNote "Används i Libris katalogiseringsverktyg för att stödja arbetsflödet att endast skapa en lokal beskrivning."@sv ;
    :code "compositional" .
   
:dependent a skos:Collection ;
    rdfs:label "dependent"@en, "avhängig"@sv ;
    rdfs:comment "Anges på egenskaper där en entitet inte kan existera utan en en entitet den länkar till. Entiteten tas automatiskt bort om den länkade entiteten tas bort."@sv ;
    skos:example "Egenskapen concerning"@sv ;
    :code "dependent" .

:distinct a skos:Collection ;
    rdfs:label "distinct"@en, "distinkt"@sv ;
    #TODO: rdfs:comment "Anges på egenskaper för att..."@sv ;
    #TODO: skos:example "Exempelvis ..."@sv ;
    skos:scopeNote "Används i Libris katalogiseringsverktyg för att stödja arbetsflödet att endast skapa en länkad beskrivning."@sv ;
    :code "distinct" .
    
:pending a skos:Collection;
    rdfs:label "pending"@en, "ej fastställd"@sv;
    rdfs:comment "Anges för att markera termer som icke stabila i väntan på fastställande av status."@sv ;
    skos:example "Egenskapen enumerationAndChronology som hittills inte använts i Libris praxis."@sv ;
    skos:scopeNote "Används i Libris katalogiseringsverktyg för att dölja dessa vid listning av egenskaper"@sv ;
    :code "pending" .

:heuristicIdentity a skos:Collection;
    rdfs:label "heuristicIdentity"@en, "heuristisk identitet"@sv;
    rdfs:comment "Anges för att markera klasser där blanka noder kan identifieras via en :heuristicIdentifier."@sv ;
    skos:example "Role, Country och Language kan identifieras via code, prefLabelByLang, altLabel osv."@sv ;
    skos:scopeNote "Används i XL för att automatiskt ersätta blanka noder med länkar"@sv ;
    :code "heuristicIdentity" .

:heuristicIdentifier a skos:Collection;
    rdfs:label "heuristicIdentifier"@en, "heuristisk identifierare"@sv;
    rdfs:comment "Anges för att markera egenskaper som kan identifiera blanka noder."@sv ;
    skos:example "prefLabelByLang, altLabel, labelByLang osv."@sv ;
    skos:scopeNote "Används i XL för att automatiskt ersätta blanka noder med länkar"@sv ;
    :code "heuristicIdentifier" .

:integral a skos:Collection ;
    rdfs:label "integral relation"@en, "väsentlig relation"@sv ;
    rdfs:comment "Anges som kategori på relationer som är väsentliga för att ge en komplett förståelse för en resurs."@sv ;
    skos:example "instanceOf, translationOf, locatedIn"@sv ;
    skos:scopeNote "Används i XL för att presentera relaterade resurser tillsammans med huvudsaklig resurs."@sv ;
    :code "integral" .


##
# Common Properties
# .. use rdfs:range rdf:langString where applicable?

:label a owl:DatatypeProperty;
    rdfs:label "label"@en, "benämning"@sv;
    rdfs:domain :Resource ;
    :category :heuristicIdentifier ;
    owl:equivalentProperty rdfs:label, sdo:name .

:singularLabel a owl:DatatypeProperty;
    rdfs:label "singular label"@en, "benämning i singular"@sv;
    rdfs:domain :Resource ;
    #:category :heuristicIdentifier ;
    rdfs:subPropertyOf :label .

:pluralLabel a owl:DatatypeProperty;
    rdfs:label "plural label"@en, "benämning i plural"@sv;
    rdfs:domain :Resource ;
    #:category :heuristicIdentifier ;
    rdfs:subPropertyOf :label .

:comment a owl:DatatypeProperty;
    rdfs:label "comment"@en, "kommentar"@sv;
    sdo:domainIncludes :Agent, :Title, :ToCEntry, :EAN, :UPC, :Language, :Script , :ChangeNote, :AdministrativeAction, bulk:Job;
    owl:equivalentProperty rdfs:comment .

:code a owl:DatatypeProperty;
    rdfs:label "kod"@sv;
    skos:altLabel "notation"@sv;
    skos:related :label;
    # sdo:domainIncludes :Concept ;
    rdfs:domain :Resource;
    :category :heuristicIdentifier ;
    owl:equivalentProperty bf2:code, skos:notation, madsrdf:code .

:count a owl:DatatypeProperty;
    rdfs:label "Number of units"@en, "Antal enheter"@sv;
    rdfs:range rdfs:Literal;
    owl:equivalentProperty bf2:count .

:Unit a owl:Class;
    rdfs:label "Unit"@en, "Enhet"@sv;
    owl:equivalentClass bf2:Unit .

:unit a owl:ObjectProperty;
    rdfs:label "Type of unit"@en, "Typ av enhet"@sv;
    rdfs:range :Unit;
    owl:equivalentProperty bf2:unit .

:value a owl:DatatypeProperty;
    rdfs:label "value"@en, "värde"@sv;
    rdfs:domain :Resource;
    owl:equivalentProperty rdf:value .

:seeAlso a owl:ObjectProperty;
    rdfs:label "see also"@en, "se även"@sv;
    rdfs:domain :Resource;
    rdfs:range :Resource;
    rdfs:subPropertyOf rdfs:seeAlso ;
    owl:equivalentProperty madsrdf:see .
# Range restrictions:
:Concept rdfs:subClassOf [ a owl:Restriction;
            owl:onProperty :seeAlso;
            owl:allValuesFrom :Concept ] .
:Agent rdfs:subClassOf [ a owl:Restriction;
            owl:onProperty :seeAlso;
            owl:allValuesFrom :BibliographicAgent ] .
:Work rdfs:subClassOf [ a owl:Restriction;
            owl:onProperty :seeAlso;
            owl:allValuesFrom :Work ] .

:sameAs a owl:ObjectProperty;
    rdfs:label "same as"@en, "samma sak som"@sv;
    owl:equivalentProperty owl:sameAs .

#:name a owl:DatatypeProperty;
#    rdfs:label "name"@en, "namn"@sv;
#    rdfs:subPropertyOf :label;
#    owl:equivalentProperty sdo:name .

:Date a rdfs:Datatype;
    owl:sameAs xsd:date .
:Time a rdfs:Datatype;
    owl:sameAs xsd:time .
:DateTime a rdfs:Datatype;
    owl:sameAs xsd:dateTime .
:Year a rdfs:Datatype;
    owl:sameAs xsd:gYear .
:Month a rdfs:Datatype;
    owl:sameAs xsd:gMonth .
:Day a rdfs:Datatype;
    owl:sameAs xsd:gDay .
:YearMonth a rdfs:Datatype;
    owl:sameAs xsd:gYearMonth .
:MonthDay a rdfs:Datatype;
    owl:sameAs xsd:gMonthDay .

:AnyDateTime a rdfs:Datatype;
    rdfs:comment "Used for dates, dates and times, and intervals."@en;
    owl:equivalentClass edtf:EDTF-level0 .
:ApproxDateTime a rdfs:Datatype;
    rdfs:comment "Used for approximate or unspecified dates, dates and times, and intervals."@en;
    owl:equivalentClass edtf:EDTF-level1 .
:PartialDateTime a rdfs:Datatype;
    rdfs:comment "Used for dates, dates and times, and intervals combining precise elements with uncertain, approximate, or unspecified parts. Also applicable for sets of dates."@en;
    owl:equivalentClass edtf:EDTF-level2 .


##
# Ambiguity (See what we do here? Reifying the unbound? Really? Proceed with care.)

:Ambiguity a owl:Class;
    rdfs:label "Ambiguity"@en, "Otydlighet"@sv;
    rdfs:comment "An ambiguous group of things sharing similar characteristics."@en .

:maybe a owl:ObjectProperty;
    rdfs:domain :Ambiguity;
    rdfs:range owl:Thing;
    rdfs:label "may be"@en, "kan vara"@sv;
    rdfs:comment "A thing that something ambiguous may be."@en .

:disambiguates a owl:ObjectProperty;
    owl:inverseOf :maybe;
    rdfs:domain owl:Thing;
    rdfs:range :Ambiguity;
    rdfs:label "disambiguates"@en, "disambiguerar"@sv;
    rdfs:comment "Something ambiguous that may be this distinct thing."@en .
